providers/evercrypt/fst/EverCrypt.HMAC.fst
@@ -54,8 +54,7 @@ val compute_blake2b: compute_st Blake2B
 
 let compute_sha1 =
   let open Hacl.Hash.SHA1 in
-  mk_compute (|SHA1, ()|) legacy_hash legacy_alloca legacy_init legacy_update_multi
-             legacy_update_last legacy_finish
+  mk_compute (|SHA1, ()|) hash alloca init update_multi update_last finish
 
 (* This implementation calls into EverCrypt.Hash, which multiplexes
    between Hacl and Vale implementations of SHA2_256 functions depending on
